Each process has its own state.

lunarlander_sl/BigStepSimple.thy
@@ -5,7 +5,7 @@ begin
 subsection \<open>Syntax\<close>
 
 text \<open>State\<close>
-type_synonym state = "char \<Rightarrow> real option"
+type_synonym state = "char \<Rightarrow> real"
 
 text \<open>Expressions\<close>
 type_synonym exp = "state \<Rightarrow> real"
@@ -43,8 +43,33 @@ datatype comm =
   Send cname exp         ("_[!]_" [110,108] 100)
 | Receive cname var     ("_[?]_" [110,108] 100)
 
+text \<open>Definition of ODEs\<close>
+
+type_synonym vec = "real^(var)"
+
+text \<open>Conversion between state and vector\<close>
+definition state2vec :: "state \<Rightarrow> vec" where
+  "state2vec s = (\<chi> x. s x)"
+
+definition vec2state :: "vec \<Rightarrow> state" where
+  "(vec2state v) x = v $ x"
+
+lemma vec_state_map1[simp]: "vec2state (state2vec s) = s"
+  unfolding vec2state_def state2vec_def by auto
+
+lemma vec_state_map2[simp]: "state2vec (vec2state s) = s"
+  unfolding vec2state_def state2vec_def by auto
+
 datatype ODE =
   ODE "var \<Rightarrow> exp"
+
+text \<open>Given ODE and a state, find the derivative vector.\<close>
+fun ODE2Vec :: "ODE \<Rightarrow> state \<Rightarrow> vec" where
+  "ODE2Vec (ODE f) s = state2vec (\<lambda>a. f a s)"
+
+text \<open>History p on time {0 .. d} is a solution to ode.\<close>
+definition ODEsol :: "ODE \<Rightarrow> (real \<Rightarrow> state) \<Rightarrow> real \<Rightarrow> bool" where
+  "ODEsol ode p d = (d \<ge> 0 \<and> (((\<lambda>t. state2vec (p t)) has_vderiv_on (\<lambda>t. ODE2Vec ode (p t))) {0 .. d}))"
 
 text \<open>HCSP processes\<close>
 datatype proc =
@@ -62,7 +87,7 @@ datatype proc =
 
 text \<open>Parallel of several HCSP processes\<close>
 datatype pproc =
-  Single "var set" proc
+  Single proc
 | Parallel pproc "cname set" pproc
 
 text \<open>Events\<close>
@@ -71,6 +96,10 @@ datatype event =
 | Out cname real 
 | IO cname real 
 
+text \<open>Global states\<close>
+datatype gstate =
+  State (single_st: state)
+| ParState (left_st: gstate) (right_st: gstate)
 
 subsection \<open>Traces\<close>
 
@@ -80,7 +109,7 @@ datatype trace_block =
   InBlock cname real
   | OutBlock cname real
   | IOBlock cname real
-  | WaitBlock time "real \<Rightarrow> state" rdy_info
+  | WaitBlock time "real \<Rightarrow> gstate" rdy_info
 
 type_synonym trace = "trace_block list"
 
@@ -143,7 +172,7 @@ inductive combine_blocks :: "cname set \<Rightarrow> trace \<Rightarrow> trace \
 | combine_blocks_wait1:
   "combine_blocks comms blks1 blks2 blks \<Longrightarrow>
    compat_rdy rdy1 rdy2 \<Longrightarrow>
-   hist = restrict (\<lambda>\<tau>. hist1 \<tau> ++ hist2 \<tau>) {0..t} \<Longrightarrow>
+   hist = restrict (\<lambda>\<tau>. ParState (hist1 \<tau>) (hist2 \<tau>)) {0..t} \<Longrightarrow>
    rdy = merge_rdy rdy1 rdy2 \<Longrightarrow>
    combine_blocks comms (WaitBlock t hist1 rdy1 # blks1) (WaitBlock t hist2 rdy2 # blks2)
                   (WaitBlock t hist rdy # blks)"
@@ -151,14 +180,18 @@ inductive combine_blocks :: "cname set \<Rightarrow> trace \<Rightarrow> trace \
   "combine_blocks comms blks1 (WaitBlock (t2 - t1) (\<lambda>\<tau>. hist2 (\<tau> - t1)) rdy2 # blks2) blks \<Longrightarrow>
    compat_rdy rdy1 rdy2 \<Longrightarrow>
    t1 < t2 \<Longrightarrow>
+   hist = restrict (\<lambda>\<tau>. ParState (hist1 \<tau>) (hist2 \<tau>)) {0..t1} \<Longrightarrow>
+   rdy = merge_rdy rdy1 rdy2 \<Longrightarrow>
    combine_blocks comms (WaitBlock t1 hist1 rdy1 # blks1) (WaitBlock t2 hist2 rdy2 # blks2)
-                  (WaitBlock t1 (\<lambda>\<tau>. hist1 \<tau> ++ hist2 \<tau>) (merge_rdy rdy1 rdy2) # blks)"
+                  (WaitBlock t1 hist rdy # blks)"
 | combine_blocks_wait3:
   "combine_blocks comms (WaitBlock (t1 - t2) (\<lambda>\<tau>. hist1 (\<tau> - t2)) rdy1 # blks1) blks2 blks \<Longrightarrow>
    compat_rdy rdy1 rdy2 \<Longrightarrow>
    t1 > t2 \<Longrightarrow>
+   hist = restrict (\<lambda>\<tau>. ParState (hist1 \<tau>) (hist2 \<tau>)) {0..t2} \<Longrightarrow>
+   rdy = merge_rdy rdy1 rdy2 \<Longrightarrow>
    combine_blocks comms (WaitBlock t1 hist1 rdy1 # blks1) (WaitBlock t2 hist2 rdy2 # blks2)
-                  (WaitBlock t2 (\<lambda>\<tau>. hist1 \<tau> ++ hist2 \<tau>) (merge_rdy rdy1 rdy2) # blks)"
+                  (WaitBlock t2 hist rdy # blks)"
 
 inductive_cases combine_blocksE1: "combine_blocks comms blks1 blks2 []"
 thm combine_blocksE1
@@ -266,21 +299,21 @@ text \<open>big_step p s1 tr s2 means executing p starting from state s1 results
 in a trace tr and final state s2.\<close>
 inductive big_step :: "proc \<Rightarrow> state \<Rightarrow> trace \<Rightarrow> state \<Rightarrow> bool" where
   skipB: "big_step Skip s [] s"
-| assignB: "big_step (Assign var e) s [] (s(var := Some (e s)))"
+| assignB: "big_step (Assign var e) s [] (s(var := e s))"
 | seqB: "big_step p1 s1 tr1 s2 \<Longrightarrow>
          big_step p2 s2 tr2 s3 \<Longrightarrow>
          big_step (Seq p1 p2) s1 (tr1 @ tr2) s3"
 | condB1: "b s1 \<Longrightarrow> big_step p1 s1 tr s2 \<Longrightarrow> big_step (Cond b p1 p2) s1 tr s2"
 | condB2: "\<not> b s1 \<Longrightarrow> big_step p2 s1 tr s2 \<Longrightarrow> big_step (Cond b p1 p2) s1 tr s2"
-| waitB: "big_step (Wait d) s [WaitBlock d (restrict (\<lambda>\<tau>. s) {0..d}) ({}, {})] s"
+| waitB: "big_step (Wait d) s [WaitBlock d (restrict (\<lambda>\<tau>. State s) {0..d}) ({}, {})] s"
 | sendB1: "big_step (Cm (Send ch e)) s [OutBlock ch (e s)] s"
 | sendB2: "d > 0 \<Longrightarrow> big_step (Cm (ch[!]e)) s
-            [WaitBlock d (restrict (\<lambda>\<tau>. s) {0..d}) ({ch}, {}),
+            [WaitBlock d (restrict (\<lambda>\<tau>. State s) {0..d}) ({ch}, {}),
              OutBlock ch (e s)] s"
-| receiveB1: "big_step (Cm (Receive ch var)) s [InBlock ch v] (s(var := Some v))"
+| receiveB1: "big_step (Cm (Receive ch var)) s [InBlock ch v] (s(var := v))"
 | receiveB2: "d > 0 \<Longrightarrow> big_step (Cm (ch[?]var)) s
-            [WaitBlock d (restrict (\<lambda>\<tau>. s) {0..d}) ({}, {ch}),
-             InBlock ch v] (s(var := Some v))"
+            [WaitBlock d (restrict (\<lambda>\<tau>. State s) {0..d}) ({}, {ch}),
+             InBlock ch v] (s(var := v))"
 | IChoiceB1: "big_step p1 s1 tr s2 \<Longrightarrow> big_step (IChoice p1 p2) s1 tr s2"
 | IChoiceB2: "big_step p2 s1 tr s2 \<Longrightarrow> big_step (IChoice p1 p2) s1 tr s2"
 | EChoiceSendB1: "i < length cs \<Longrightarrow> cs ! i = (Send ch e, p2) \<Longrightarrow>
@@ -288,14 +321,14 @@ inductive big_step :: "proc \<Rightarrow> state \<Rightarrow> trace \<Rightarrow
     big_step (EChoice cs) s1 (OutBlock ch (e s1) # tr2) s2"
 | EChoiceSendB2: "d > 0 \<Longrightarrow> i < length cs \<Longrightarrow> cs ! i = (Send ch e, p2) \<Longrightarrow>
     big_step p2 s1 tr2 s2 \<Longrightarrow>
-    big_step (EChoice cs) s1 (WaitBlock d (restrict (\<lambda>\<tau>. s1) {0..d}) (rdy_of_echoice cs) #
+    big_step (EChoice cs) s1 (WaitBlock d (restrict (\<lambda>\<tau>. State s1) {0..d}) (rdy_of_echoice cs) #
                               OutBlock ch (e s1) # tr2) s2"
 | EChoiceReceiveB1: "i < length cs \<Longrightarrow> cs ! i = (Receive ch var, p2) \<Longrightarrow>
-    big_step p2 (s1(var := Some v)) tr2 s2 \<Longrightarrow>
+    big_step p2 (s1(var := v)) tr2 s2 \<Longrightarrow>
     big_step (EChoice cs) s1 (InBlock ch v # tr2) s2"
 | EChoiceReceiveB2: "d > 0 \<Longrightarrow> i < length cs \<Longrightarrow> cs ! i = (Receive ch var, p2) \<Longrightarrow>
-    big_step p2 (s1(var := Some v)) tr2 s2 \<Longrightarrow>
-    big_step (EChoice cs) s1 (WaitBlock d (restrict (\<lambda>\<tau>. s1) {0..d}) (rdy_of_echoice cs) #
+    big_step p2 (s1(var := v)) tr2 s2 \<Longrightarrow>
+    big_step (EChoice cs) s1 (WaitBlock d (restrict (\<lambda>\<tau>. State s1) {0..d}) (rdy_of_echoice cs) #
                               InBlock ch v # tr2) s2"
 | RepetitionB1: "big_step (Rep p) s [] s"
 | RepetitionB2: "big_step p s1 tr1 s2 \<Longrightarrow> big_step (Rep p) s2 tr2 s3 \<Longrightarrow>
@@ -305,40 +338,33 @@ inductive big_step :: "proc \<Rightarrow> state \<Rightarrow> trace \<Rightarrow
 | ContB2: "d > 0 \<Longrightarrow> ODEsol ode p d \<Longrightarrow>
      (\<forall>t. t \<ge> 0 \<and> t < d \<longrightarrow> b (p t)) \<Longrightarrow>
      \<not>b (p d) \<Longrightarrow> p 0 = s1 \<Longrightarrow>
-     big_step (Cont ode b) s1 [WaitBlock d (restrict p {0..d}) ({}, {})] (p d)"
+     big_step (Cont ode b) s1 [WaitBlock d (restrict (\<lambda>\<tau>. State (p \<tau>)) {0..d}) ({}, {})] (p d)"
 | InterruptSendB1: "i < length cs \<Longrightarrow> cs ! i = (Send ch e, p2) \<Longrightarrow>
     big_step p2 s1 tr2 s2 \<Longrightarrow>
     big_step (Interrupt ode cs) s1 (OutBlock ch (e s) # tr2) s2"
 | InterruptSendB2: "d > 0 \<Longrightarrow> ODEsol ode p d \<Longrightarrow> p 0 = s1 \<Longrightarrow>
     i < length cs \<Longrightarrow> cs ! i = (Send ch e, p2) \<Longrightarrow>
     big_step p2 (p d) tr2 s2 \<Longrightarrow>
-    big_step (Interrupt ode cs) s1 (WaitBlock d (restrict p {0..d}) (rdy_of_echoice cs) #
+    big_step (Interrupt ode cs) s1 (WaitBlock d (restrict (\<lambda>\<tau>. State (p \<tau>)) {0..d}) (rdy_of_echoice cs) #
                                     OutBlock ch (e s) # tr) s2"
 | InterruptReceiveB1: "i < length cs \<Longrightarrow> cs ! i = (Receive ch var, p2) \<Longrightarrow>
-    big_step p2 (s1(var := Some v)) tr2 s2 \<Longrightarrow>
+    big_step p2 (s1(var := v)) tr2 s2 \<Longrightarrow>
     big_step (Interrupt ode cs) s1 (InBlock ch v # tr2) s2"
 | InterruptReceiveB2: "d > 0 \<Longrightarrow> ODEsol ode p d \<Longrightarrow> p 0 = s1 \<Longrightarrow>
     i < length cs \<Longrightarrow> cs ! i = (Receive ch var, p2) \<Longrightarrow>
-    big_step p2 ((p d)(var := Some v)) tr2 s2 \<Longrightarrow>
-    big_step (Interrupt ode cs) s1 (WaitBlock d (restrict p {0..d}) (rdy_of_echoice cs) #
+    big_step p2 ((p d)(var := v)) tr2 s2 \<Longrightarrow>
+    big_step (Interrupt ode cs) s1 (WaitBlock d (restrict (\<lambda>\<tau>. State (p \<tau>)) {0..d}) (rdy_of_echoice cs) #
                                     InBlock ch v # tr2) s2"
 
 text \<open>Big-step semantics for parallel processes.\<close>
 
-fun vars_of_pproc :: "pproc \<Rightarrow> var set" where
-  "vars_of_pproc (Single vars _) = vars"
-| "vars_of_pproc (Parallel p1 chs p2) = vars_of_pproc p1 \<union> vars_of_pproc p2"
-
-
-inductive par_big_step :: "pproc \<Rightarrow> state \<Rightarrow> trace \<Rightarrow> state \<Rightarrow> bool" where
-  SingleB: "big_step p s1 tr s2 \<Longrightarrow> par_big_step (Single vars p) s1 tr s2"
+inductive par_big_step :: "pproc \<Rightarrow> gstate \<Rightarrow> trace \<Rightarrow> gstate \<Rightarrow> bool" where
+  SingleB: "big_step p s1 tr s2 \<Longrightarrow> par_big_step (Single p) (State s1) tr (State s2)"
 | ParallelB:
-    "par_big_step p1 (restrict_map s1 (vars_of_pproc p1)) tr1 s12 \<Longrightarrow>
-     par_big_step p2 (restrict_map s1 (vars_of_pproc p2)) tr2 s22 \<Longrightarrow>
+    "par_big_step p1 s11 tr1 s12 \<Longrightarrow>
+     par_big_step p2 s12 tr2 s22 \<Longrightarrow>
      combine_blocks chs tr1 tr2 tr \<Longrightarrow>
-     s12 = restrict_map s2 (vars_of_pproc p1) \<Longrightarrow>
-     s22 = restrict_map s2 (vars_of_pproc p2) \<Longrightarrow>
-     par_big_step (Parallel p1 chs p2) s1 tr s2"
+     par_big_step (Parallel p1 chs p2) (ParState s11 s12) tr (ParState s12 s22)"
 
 subsection \<open>More convenient version of rules\<close>
 
@@ -358,72 +384,76 @@ subsection \<open>Test of big-step semantics\<close>
 
 text \<open>Send 1 immediately\<close>
 lemma test1a: "big_step (Cm (''ch''[!](\<lambda>_. 1)))
-  Map.empty [OutBlock ''ch'' 1] Map.empty"
+  (\<lambda>_. 0) [OutBlock ''ch'' 1] (\<lambda>_. 0)"
   by (rule sendB1)
 
 text \<open>Send x + 1 immediately\<close>
-lemma test1b: "big_step (Cm (''ch''[!](\<lambda>s. the (s X) + 1)))
-  ([X \<mapsto> 1]) [OutBlock ''ch'' 2] ([X \<mapsto> 1])"
+lemma test1b: "big_step (Cm (''ch''[!](\<lambda>s. s X + 1)))
+  ((\<lambda>_. 0)(X := 1)) [OutBlock ''ch'' 2] ((\<lambda>_. 0)(X := 1))"
   by (rule sendB1', auto)
 
 text \<open>Send 1 after delay 2\<close>
 lemma test1c: "big_step (Cm (''ch''[!](\<lambda>_. 1)))
-  Map.empty [WaitBlock 2 (restrict (\<lambda>_. Map.empty) {0..2}) ({''ch''}, {}),
-             OutBlock ''ch'' 1] Map.empty"
+  (\<lambda>_. 0) [WaitBlock 2 (restrict (\<lambda>_. State (\<lambda>_. 0)) {0..2}) ({''ch''}, {}),
+           OutBlock ''ch'' 1] (\<lambda>_. 0)"
   by (rule sendB2, auto)
 
 text \<open>Receive 1 immediately\<close>
 lemma test2a: "big_step (Cm (''ch''[?]X))
-  Map.empty [InBlock ''ch'' 1] ([X \<mapsto> 1])"
+  (\<lambda>_. 0) [InBlock ''ch'' 1] ((\<lambda>_. 0)(X := 1))"
   by (rule receiveB1)
 
 text \<open>Receive 1 after delay 2\<close>
 lemma test2b: "big_step (Cm (''ch''[?]X))
-  Map.empty [WaitBlock 2 (restrict (\<lambda>_. Map.empty) {0..2}) ({}, {''ch''}),
-             InBlock ''ch'' 1] ([X \<mapsto> 1])"
+  (\<lambda>_. 0) [WaitBlock 2 (restrict (\<lambda>_. State (\<lambda>_. 0)) {0..2}) ({}, {''ch''}),
+           InBlock ''ch'' 1] ((\<lambda>_. 0)(X := 1))"
   by (rule receiveB2, auto)
 
 text \<open>Communication\<close>
 lemma test3: "par_big_step (
-  Parallel (Single {} (Cm (''ch''[!](\<lambda>_. 1)))) {''ch''}
-           (Single {X} (Cm (''ch''[?]X))))
-  Map.empty [IOBlock ''ch'' 1] ([X \<mapsto> 1])"
+  Parallel (Single (Cm (''ch''[!](\<lambda>_. 1)))) {''ch''}
+           (Single (Cm (''ch''[?]X))))
+  (ParState (State (\<lambda>_. 0)) (State (\<lambda>_. 0)))
+    [IOBlock ''ch'' 1]
+  (ParState (State (\<lambda>_. 0)) (State ((\<lambda>_. 0)(X := 1))))"
   apply (rule ParallelB)
-     apply auto apply (rule SingleB[OF test1a])
-    apply (rule SingleB[OF test2a])
+    apply (rule SingleB[OF test1a])
+   apply (rule SingleB[OF test2a])
   by (auto intro: combine_blocks.intros)
 
 text \<open>Wait\<close>
 lemma test4: "big_step (Wait 2)
-  Map.empty [WaitBlock 2 (restrict (\<lambda>_. Map.empty) {0..2}) ({}, {})] Map.empty"
+  (\<lambda>_. 0) [WaitBlock 2 (restrict (\<lambda>_. State (\<lambda>_. 0)) {0..2}) ({}, {})] (\<lambda>_. 0)"
   by (rule waitB)
 
 text \<open>Seq\<close>
 lemma test5: "big_step (Wait 2; Cm (''ch''[!](\<lambda>_. 1)))
-  Map.empty [WaitBlock 2 (restrict (\<lambda>_. Map.empty) {0..2}) ({}, {}), OutBlock ''ch'' 1] Map.empty"
+  (\<lambda>_. 0) [WaitBlock 2 (restrict (\<lambda>_. State (\<lambda>_. 0)) {0..2}) ({}, {}), OutBlock ''ch'' 1] (\<lambda>_. 0)"
   by (rule seqB'[OF test4 test1a], auto)
 
 text \<open>Communication after delay 2\<close>
 lemma test6: "par_big_step (
-  Parallel (Single {} (Wait 2; Cm (''ch''[!](\<lambda>_. 1)))) {''ch''}
-           (Single {X} (Cm (''ch''[?]X))))
-  Map.empty [WaitBlock 2 (restrict (\<lambda>_. Map.empty) {0..2}) ({}, {''ch''}), IOBlock ''ch'' 1] ([X \<mapsto> 1])"
+  Parallel (Single (Wait 2; Cm (''ch''[!](\<lambda>_. 1)))) {''ch''}
+           (Single (Cm (''ch''[?]X))))
+  (ParState (State (\<lambda>_. 0)) (State (\<lambda>_. 0)))
+    [WaitBlock 2 (restrict (\<lambda>_. ParState (State (\<lambda>_. 0)) (State (\<lambda>_. 0))) {0..2}) ({}, {''ch''}), IOBlock ''ch'' 1]
+  (ParState (State (\<lambda>_. 0)) (State ((\<lambda>_. 0)(X := 1))))"
   apply (rule ParallelB)
-     apply auto apply (rule SingleB[OF test5])
-    apply (rule SingleB[OF test2b])
+    apply (rule SingleB[OF test5])
+   apply (rule SingleB[OF test2b])
   by (auto intro!: combine_blocks.intros)
 
 text \<open>Loop one time\<close>
-lemma test7: "big_step (Rep (Assign X (\<lambda>s. the (s X) + 1); Cm (''ch''[!](\<lambda>s. the (s X)))))
-  ([X \<mapsto> 0]) [OutBlock ''ch'' 1] ([X \<mapsto> 1])"
+lemma test7: "big_step (Rep (Assign X (\<lambda>s. s X + 1); Cm (''ch''[!](\<lambda>s. s X))))
+  (\<lambda>_. 0) [OutBlock ''ch'' 1] ((\<lambda>_. 0)(X := 1))"
   apply (rule RepetitionB2)
     apply (rule seqB) apply (rule assignB) apply (rule sendB1)
   apply auto[1] apply (rule RepetitionB1)
   by auto
 
 text \<open>Loop two times\<close>
-lemma test8: "big_step (Rep (Assign X (\<lambda>s. the (s X) + 1); Cm (''ch''[!](\<lambda>s. the (s X)))))
-  ([X \<mapsto> 0]) [OutBlock ''ch'' 1, OutBlock ''ch'' 2] ([X \<mapsto> 2])"
+lemma test8: "big_step (Rep (Assign X (\<lambda>s. s X + 1); Cm (''ch''[!](\<lambda>s. s X))))
+  (\<lambda>_. 0) [OutBlock ''ch'' 1, OutBlock ''ch'' 2] ((\<lambda>_. 0)(X := 2))"
   apply (rule RepetitionB2)
     apply (rule seqB) apply (rule assignB) apply (rule sendB1)
    apply auto[1] apply (rule RepetitionB2)
@@ -434,28 +464,30 @@ lemma test8: "big_step (Rep (Assign X (\<lambda>s. the (s X) + 1); Cm (''ch''[!]
 text \<open>External choice 1\<close>
 lemma test9a: "big_step (EChoice [(''ch1''[!](\<lambda>_. 1), Wait 1),
                                   (''ch2''[!](\<lambda>_. 2), Wait 2)])
-  Map.empty [OutBlock ''ch1'' 1, WaitBlock 1 (restrict (\<lambda>_. Map.empty) {0..1}) ({}, {})] Map.empty"
+  (\<lambda>_. 0) [OutBlock ''ch1'' 1, WaitBlock 1 (restrict (\<lambda>_. State (\<lambda>_. 0)) {0..1}) ({}, {})] (\<lambda>_. 0)"
   apply (rule EChoiceSendB1[where i=0])
   apply auto by (rule waitB)
 
 text \<open>External choice 2\<close>
 lemma test9b: "big_step (EChoice [(''ch1''[!](\<lambda>_. 1), Wait 1),
                                   (''ch2''[!](\<lambda>_. 2), Wait 2)])
-  Map.empty [OutBlock ''ch2'' 2, WaitBlock 2 (restrict (\<lambda>_. Map.empty) {0..2}) ({}, {})] Map.empty"
+  (\<lambda>_. 0) [OutBlock ''ch2'' 2, WaitBlock 2 (restrict (\<lambda>_. State (\<lambda>_. 0)) {0..2}) ({}, {})] (\<lambda>_. 0)"
   apply (rule EChoiceSendB1[where i=1])
   apply auto by (rule waitB)
 
 text \<open>Communication with external choice\<close>
 lemma test10: "par_big_step (
-  Parallel (Single {} (EChoice [(''ch1''[!](\<lambda>_. 1), Wait 1),
+  Parallel (Single (EChoice [(''ch1''[!](\<lambda>_. 1), Wait 1),
                              (''ch2''[!](\<lambda>_. 2), Wait 2)])) {''ch1'', ''ch2''}
-           (Single {X} (Cm (''ch1''[?]X); Wait 1)))
-  Map.empty [IOBlock ''ch1'' 1, WaitBlock 1 (restrict (\<lambda>_. [X \<mapsto> 1]) {0..1}) ({}, {})] [X \<mapsto> 1]"
+           (Single (Cm (''ch1''[?]X); Wait 1)))
+  (ParState (State (\<lambda>_. 0)) (State (\<lambda>_. 0)))
+    [IOBlock ''ch1'' 1, WaitBlock 1 (restrict (\<lambda>_. ParState (State (\<lambda>_. 0)) (State ((\<lambda>_. 0)(X := 1)))) {0..1}) ({}, {})]
+  (ParState (State (\<lambda>_. 0)) (State ((\<lambda>_. 0)(X := 1))))"
   apply (rule ParallelB)
-     apply auto apply (rule SingleB[OF test9a])
-    apply (rule SingleB)
-    apply (rule seqB) apply (rule receiveB1) apply (rule waitB)
-   apply auto
+    apply (rule SingleB[OF test9a])
+   apply (rule SingleB)
+   apply (rule seqB) apply (rule receiveB1) apply (rule waitB)
+  apply auto
   by (intro combine_blocks.intros, auto)
 
 subsection \<open>Validity\<close>
@@ -508,7 +540,7 @@ theorem Valid_skip:
 
 theorem Valid_assign:
   "Valid
-    (\<lambda>s tr. Q (s(var \<mapsto> e s)) tr)
+    (\<lambda>s tr. Q (s(var := e s)) tr)
     (Assign var e)
     Q"
   unfolding Valid_def
@@ -517,7 +549,7 @@ theorem Valid_assign:
 theorem Valid_send:
   "Valid
     (\<lambda>s tr. Q s (tr @ [OutBlock ch (e s)]) \<and>
-        (\<forall>d>0. Q s (tr @ [WaitBlock d (\<lambda>\<tau>\<in>{0..d}. s) ({ch}, {}), OutBlock ch (e s)])))
+        (\<forall>d>0. Q s (tr @ [WaitBlock d (\<lambda>\<tau>\<in>{0..d}. State s) ({ch}, {}), OutBlock ch (e s)])))
     (Cm (ch[!]e))
     Q"
   unfolding Valid_def
@@ -525,8 +557,8 @@ theorem Valid_send:
 
 theorem Valid_receive:
   "Valid
-    (\<lambda>s tr. (\<forall>v. Q (s(var := Some v)) (tr @ [InBlock ch v])) \<and>
-        (\<forall>d>0. \<forall>v. Q (s(var := Some v)) (tr @ [WaitBlock d (\<lambda>\<tau>\<in>{0..d}. s) ({}, {ch}), InBlock ch v])))
+    (\<lambda>s tr. (\<forall>v. Q (s(var := v)) (tr @ [InBlock ch v])) \<and>
+        (\<forall>d>0. \<forall>v. Q (s(var := v)) (tr @ [WaitBlock d (\<lambda>\<tau>\<in>{0..d}. State s) ({}, {ch}), InBlock ch v])))
     (Cm (ch[?]var))
     Q"
   unfolding Valid_def
@@ -539,7 +571,7 @@ theorem Valid_seq:
 
 theorem Valid_wait:
   "Valid
-    (\<lambda>s tr. Q s (tr @ [WaitBlock d (\<lambda>\<tau>\<in>{0..d}. s) ({}, {})]))
+    (\<lambda>s tr. Q s (tr @ [WaitBlock d (\<lambda>\<tau>\<in>{0..d}. State s) ({}, {})]))
     (Wait d)
     Q"
   unfolding Valid_def
@@ -571,11 +603,11 @@ theorem Valid_echoice:
       (ch[!]e, p2) \<Rightarrow>
         (\<exists>Q. Valid Q p2 R \<and> (P \<Longrightarrow>\<^sub>A (\<lambda>s tr. 
             Q s (tr @ [OutBlock ch (e s)]) \<and>
-            (\<forall>d>0. Q s (tr @ [WaitBlock d (\<lambda>\<tau>\<in>{0..d}. s) (rdy_of_echoice es), OutBlock ch (e s)])))))
+            (\<forall>d>0. Q s (tr @ [WaitBlock d (\<lambda>\<tau>\<in>{0..d}. State s) (rdy_of_echoice es), OutBlock ch (e s)])))))
     | (ch[?]var, p2) \<Rightarrow>
         (\<exists>Q. Valid Q p2 R \<and> (P \<Longrightarrow>\<^sub>A (\<lambda>s tr.
-            (\<forall>v. Q (s(var := Some v)) (tr @ [InBlock ch v])) \<and>
-            (\<forall>d>0. \<forall>v. Q (s(var := Some v)) (tr @ [WaitBlock d (\<lambda>\<tau>\<in>{0..d}. s) (rdy_of_echoice es), InBlock ch v])))))"
+            (\<forall>v. Q (s(var := v)) (tr @ [InBlock ch v])) \<and>
+            (\<forall>d>0. \<forall>v. Q (s(var := v)) (tr @ [WaitBlock d (\<lambda>\<tau>\<in>{0..d}. State s) (rdy_of_echoice es), InBlock ch v])))))"
   shows "Valid P (EChoice es) R"
 proof -
   have a: "R s2 (tr1 @ tr2)" if *: "P s1 tr1" "tr2 = OutBlock ch (e s1) # tr2a" "i < length es" "es ! i = (ch[!]e, p2)"
@@ -584,7 +616,7 @@ proof -
   proof -
     from assms obtain Q where 1:
       "Valid Q p2 R"
-      "P \<Longrightarrow>\<^sub>A (\<lambda>s tr. Q s (tr @ [OutBlock ch (e s)]) \<and> (\<forall>d>0. Q s (tr @ [WaitBlock d (\<lambda>\<tau>\<in>{0..d}. s) (rdy_of_echoice es), OutBlock ch (e s)])))"
+      "P \<Longrightarrow>\<^sub>A (\<lambda>s tr. Q s (tr @ [OutBlock ch (e s)]) \<and> (\<forall>d>0. Q s (tr @ [WaitBlock d (\<lambda>\<tau>\<in>{0..d}. State s) (rdy_of_echoice es), OutBlock ch (e s)])))"
       using *(3,4) by fastforce
     have 2: "Q s1 (tr1 @ [OutBlock ch (e s1)])"
       using 1(2) *(1) unfolding entails_def by auto
@@ -593,47 +625,50 @@ proof -
     then show ?thesis
       using *(2) by auto
   qed
-  have b: "R s2 (tr1 @ tr2)" if *: "P s1 tr1" "tr2 = WaitBlock d (\<lambda>\<tau>\<in>{0..d}. s1) (rdy_of_echoice es) # OutBlock ch (e s1) # tr2a"
+  have b: "R s2 (tr1 @ tr2)" if *: "P s1 tr1" "tr2 = WaitBlock d (\<lambda>\<tau>\<in>{0..d}. State s1) (rdy_of_echoice es) # OutBlock ch (e s1) # tr2a"
       "0 < d" "i < length es" "es ! i = (ch[!]e, p2)" "big_step p2 s1 tr2a s2"
     for s1 tr1 s2 tr2 d i ch e p2 tr2a
   proof -
     from assms obtain Q where 1:
       "Valid Q p2 R"
-      "P \<Longrightarrow>\<^sub>A (\<lambda>s tr. Q s (tr @ [OutBlock ch (e s)]) \<and> (\<forall>d>0. Q s (tr @ [WaitBlock d (\<lambda>\<tau>\<in>{0..d}. s) (rdy_of_echoice es), OutBlock ch (e s)])))"
+      "P \<Longrightarrow>\<^sub>A (\<lambda>s tr. Q s (tr @ [OutBlock ch (e s)]) \<and>
+                     (\<forall>d>0. Q s (tr @ [WaitBlock d (\<lambda>\<tau>\<in>{0..d}. State s) (rdy_of_echoice es), OutBlock ch (e s)])))"
       using *(4,5) by fastforce
-    have 2: "Q s1 (tr1 @ [WaitBlock d (\<lambda>\<tau>\<in>{0..d}. s1) (rdy_of_echoice es), OutBlock ch (e s1)])"
+    have 2: "Q s1 (tr1 @ [WaitBlock d (\<lambda>\<tau>\<in>{0..d}. State s1) (rdy_of_echoice es), OutBlock ch (e s1)])"
       using 1(2) *(1,3) unfolding entails_def by auto
-    have 3: "R s2 (tr1 @ [WaitBlock d (\<lambda>\<tau>\<in>{0..d}. s1) (rdy_of_echoice es), OutBlock ch (e s1)] @ tr2a)"
+    have 3: "R s2 (tr1 @ [WaitBlock d (\<lambda>\<tau>\<in>{0..d}. State s1) (rdy_of_echoice es), OutBlock ch (e s1)] @ tr2a)"
       using *(6) 1(1) 2 unfolding Valid_def by fastforce
     then show ?thesis
       using *(2) by auto
   qed
   have c: "R s2 (tr1 @ tr2)" if *: "P s1 tr1" "tr2 = InBlock ch v # tr2a" "i < length es" "es ! i = (ch[?]var, p2)"
-      "big_step p2 (s1(var \<mapsto> v)) tr2a s2"
+      "big_step p2 (s1(var := v)) tr2a s2"
     for s1 tr1 s2 tr2 i ch var p2 v tr2a
   proof -
     from assms obtain Q where 1:
       "Valid Q p2 R"
-      "P \<Longrightarrow>\<^sub>A (\<lambda>s tr. (\<forall>v. Q (s(var := Some v)) (tr @ [InBlock ch v]) )\<and> (\<forall>d>0. \<forall>v. Q (s(var := Some v)) (tr @ [WaitBlock d (\<lambda>\<tau>\<in>{0..d}. s) (rdy_of_echoice es), InBlock ch v])))"
+      "P \<Longrightarrow>\<^sub>A (\<lambda>s tr. (\<forall>v. Q (s(var := v)) (tr @ [InBlock ch v])) \<and>
+                      (\<forall>d>0. \<forall>v. Q (s(var := v)) (tr @ [WaitBlock d (\<lambda>\<tau>\<in>{0..d}. State s) (rdy_of_echoice es), InBlock ch v])))"
       using *(3,4) by fastforce
-    have 2: "Q (s1(var := Some v)) (tr1 @ [InBlock ch v])"
+    have 2: "Q (s1(var := v)) (tr1 @ [InBlock ch v])"
       using 1(2) *(1) unfolding entails_def by auto
     have 3: "R s2 (tr1 @ [InBlock ch v] @ tr2a)"
       using *(5) 1(1) 2 unfolding Valid_def by fastforce
     then show ?thesis
       using *(2) by auto
   qed
-  have d: "R s2 (tr1 @ tr2)" if *: "P s1 tr1" "tr2 = WaitBlock d (\<lambda>\<tau>\<in>{0..d}. s1) (rdy_of_echoice es) # InBlock ch v # tr2a"
-      "0 < d" "i < length es" "es ! i = (ch[?]var, p2)" "big_step p2 (s1(var \<mapsto> v)) tr2a s2"
+  have d: "R s2 (tr1 @ tr2)" if *: "P s1 tr1" "tr2 = WaitBlock d (\<lambda>\<tau>\<in>{0..d}. State s1) (rdy_of_echoice es) # InBlock ch v # tr2a"
+      "0 < d" "i < length es" "es ! i = (ch[?]var, p2)" "big_step p2 (s1(var := v)) tr2a s2"
     for s1 tr1 s2 tr2 d i ch var p2 v tr2a
   proof -
     from assms obtain Q where 1:
       "Valid Q p2 R"
-      "P \<Longrightarrow>\<^sub>A (\<lambda>s tr. (\<forall>v. Q (s(var := Some v)) (tr @ [InBlock ch v]) )\<and> (\<forall>d>0. \<forall>v. Q (s(var := Some v)) (tr @ [WaitBlock d (\<lambda>\<tau>\<in>{0..d}. s) (rdy_of_echoice es), InBlock ch v])))"
+      "P \<Longrightarrow>\<^sub>A (\<lambda>s tr. (\<forall>v. Q (s(var := v)) (tr @ [InBlock ch v])) \<and>
+                      (\<forall>d>0. \<forall>v. Q (s(var := v)) (tr @ [WaitBlock d (\<lambda>\<tau>\<in>{0..d}. State s) (rdy_of_echoice es), InBlock ch v])))"
       using *(4,5) by fastforce
-    have 2: "Q (s1(var \<mapsto> v)) (tr1 @ [WaitBlock d (\<lambda>\<tau>\<in>{0..d}. s1) (rdy_of_echoice es), InBlock ch v])"
+    have 2: "Q (s1(var := v)) (tr1 @ [WaitBlock d (\<lambda>\<tau>\<in>{0..d}. State s1) (rdy_of_echoice es), InBlock ch v])"
       using 1(2) *(1,3) unfolding entails_def by auto
-    have 3: "R s2 (tr1 @ [WaitBlock d (\<lambda>\<tau>\<in>{0..d}. s1) (rdy_of_echoice es), InBlock ch v] @ tr2a)"
+    have 3: "R s2 (tr1 @ [WaitBlock d (\<lambda>\<tau>\<in>{0..d}. State s1) (rdy_of_echoice es), InBlock ch v] @ tr2a)"
       using *(6) 1(1) 2 unfolding Valid_def by fastforce
     then show ?thesis
       using *(2) by auto
@@ -649,10 +684,10 @@ theorem Valid_echoice_InIn:
   assumes "Valid Q1 p1 R"
     and "Valid Q2 p2 R"
   shows "Valid
-    (\<lambda>s tr. (\<forall>v. Q1 (s(var1 := Some v)) (tr @ [InBlock ch1 v])) \<and>
-            (\<forall>d>0. \<forall>v. Q1 (s(var1 := Some v)) (tr @ [WaitBlock d (\<lambda>\<tau>\<in>{0..d}. s) ({}, {ch1, ch2}), InBlock ch1 v])) \<and>
-            (\<forall>v. Q2 (s(var2 := Some v)) (tr @ [InBlock ch2 v])) \<and>
-            (\<forall>d>0. \<forall>v. Q2 (s(var2 := Some v)) (tr @ [WaitBlock d (\<lambda>\<tau>\<in>{0..d}. s) ({}, {ch1, ch2}), InBlock ch2 v])))
+    (\<lambda>s tr. (\<forall>v. Q1 (s(var1 := v)) (tr @ [InBlock ch1 v])) \<and>
+            (\<forall>d>0. \<forall>v. Q1 (s(var1 := v)) (tr @ [WaitBlock d (\<lambda>\<tau>\<in>{0..d}. State s) ({}, {ch1, ch2}), InBlock ch1 v])) \<and>
+            (\<forall>v. Q2 (s(var2 := v)) (tr @ [InBlock ch2 v])) \<and>
+            (\<forall>d>0. \<forall>v. Q2 (s(var2 := v)) (tr @ [WaitBlock d (\<lambda>\<tau>\<in>{0..d}. State s) ({}, {ch1, ch2}), InBlock ch2 v])))
       (EChoice [(ch1[?]var1, p1), (ch2[?]var2, p2)])
     R"
 proof -
@@ -684,11 +719,26 @@ qed
 
 subsection \<open>Validity for parallel programs\<close>
 
-definition ParValid :: "fform \<Rightarrow> pproc \<Rightarrow> assn \<Rightarrow> bool" where
+text \<open>Assertion on global state\<close>
+type_synonym gs_assn = "gstate \<Rightarrow> bool"
+
+text \<open>Assertion on global state and trace\<close>
+type_synonym gassn = "gstate \<Rightarrow> trace \<Rightarrow> bool"
+
+definition par_assn :: "gs_assn \<Rightarrow> gs_assn \<Rightarrow> gs_assn" where
+  "par_assn P Q = (\<lambda>s. P (left_st s) \<and> Q (right_st s))"
+
+definition sing_assn :: "fform \<Rightarrow> gs_assn" where
+  "sing_assn P = (\<lambda>s. P (single_st s))"
+
+definition pair_assn :: "fform \<Rightarrow> fform \<Rightarrow> gs_assn" where
+  "pair_assn P Q = par_assn (sing_assn P) (sing_assn Q)"
+
+definition ParValid :: "gs_assn \<Rightarrow> pproc \<Rightarrow> gassn \<Rightarrow> bool" where
   "ParValid P c Q \<longleftrightarrow> (\<forall>s1 s2 tr2. P s1 \<longrightarrow> par_big_step c s1 tr2 s2 \<longrightarrow> Q s2 tr2)"
 
 
-inductive_cases SingleE: "par_big_step (Single vars p) s1 tr s2"
+inductive_cases SingleE: "par_big_step (Single p) s1 tr s2"
 thm SingleE
 
 inductive_cases ParallelE: "par_big_step (Parallel p1 ch p2) s1 tr s2"
@@ -696,30 +746,27 @@ thm ParallelE
 
 lemma ParValid_Single:
   assumes "Valid P c Q"
-  shows "ParValid (\<lambda>s. P s []) (Single vars c) Q"
+  shows "ParValid (\<lambda>s. P (single_st s) []) (Single c) (\<lambda>s tr. Q (single_st s) tr)"
   using assms unfolding ParValid_def Valid_def
-  by (metis SingleE append.left_neutral)
+  by (metis SingleE append.monoid_axioms gstate.sel(1) monoid.left_neutral)
 
 lemma ParValid_Parallel:
   assumes "ParValid P1 p1 Q1"
     and "ParValid P2 p2 Q2"
-  shows "ParValid (\<lambda>s. P1 (restrict_map s (vars_of_pproc p1)) \<and>
-                       P2 (restrict_map s (vars_of_pproc p2)))
+  shows "ParValid (\<lambda>s. P1 (left_st s) \<and> P2 (right_st s))
           (Parallel p1 chs p2)
-         (\<lambda>s tr. \<exists>tr1 tr2. Q1 (restrict_map s (vars_of_pproc p1)) tr1 \<and>
-                           Q2 (restrict_map s (vars_of_pproc p2)) tr2 \<and>
-                           combine_blocks chs tr1 tr2 tr)"
+         (\<lambda>s tr. \<exists>tr1 tr2. Q1 (left_st s) tr1 \<and> Q2 (right_st s) tr2 \<and> combine_blocks chs tr1 tr2 tr)"
 proof -
-  have *: "\<exists>tr1 tr2a. Q1 (s2 |` vars_of_pproc p1) tr1 \<and> Q2 (s2 |` vars_of_pproc p2) tr2a \<and> combine_blocks chs tr1 tr2a ([] @ tr2)"
-    if "P1 (s1 |` vars_of_pproc p1)"
-       "P2 (s1 |` vars_of_pproc p2)"
-       "par_big_step p1 (s1 |` vars_of_pproc p1) tr1a (s2 |` vars_of_pproc p1)"
-       "par_big_step p2 (s1 |` vars_of_pproc p2) tr2a (s2 |` vars_of_pproc p2)"
+  have *: "\<exists>tr1 tr2a. Q1 (left_st s2) tr1 \<and> Q2 (right_st s2) tr2a \<and> combine_blocks chs tr1 tr2a ([] @ tr2)"
+    if "P1 (left_st s1)"
+       "P2 (right_st s1)"
+       "par_big_step p1 (left_st s1) tr1a (left_st s2)"
+       "par_big_step p2 (right_st s1) tr2a (right_st s2)"
        "combine_blocks chs tr1a tr2a tr2" for s1 s2 tr2 tr1a tr2a
   proof -
-    have 1: "Q1 (s2 |` vars_of_pproc p1) tr1a"
+    have 1: "Q1 (left_st s2) tr1a"
       using that(1,3) assms(1) unfolding ParValid_def by force
-    have 2: "Q2 (s2 |` vars_of_pproc p2) tr2a"
+    have 2: "Q2 (right_st s2) tr2a"
       using that(2,4) assms(2) unfolding ParValid_def by force
     show ?thesis
       apply (rule exI[where x=tr1a])
@@ -729,20 +776,17 @@ proof -
   show ?thesis
     unfolding ParValid_def apply clarify
     apply (elim ParallelE)
-    using * by auto
+    using * by (metis ParValid_def assms(1) assms(2) gstate.sel(2) gstate.sel(3))
 qed
 
 lemma ParValid_Parallel':
   assumes "ParValid P1 p1 Q1"
     and "ParValid P2 p2 Q2"
-    and "\<And>s. P s \<Longrightarrow> P1 (restrict_map s (vars_of_pproc p1)) \<and>
-                     P2 (restrict_map s (vars_of_pproc p2))"
-    and "(\<lambda>s tr. \<exists>tr1 tr2. Q1 (restrict_map s (vars_of_pproc p1)) tr1 \<and>
-                           Q2 (restrict_map s (vars_of_pproc p2)) tr2 \<and>
-                           combine_blocks chs tr1 tr2 tr) \<Longrightarrow>\<^sub>A Q"
+    and "\<And>s. P s \<Longrightarrow> P1 (left_st s) \<and> P2 (right_st s)"
+    and "\<And>s tr. (\<exists>tr1 tr2. Q1 (left_st s) tr1 \<and> Q2 (right_st s) tr2 \<and> combine_blocks chs tr1 tr2 tr) \<Longrightarrow> Q s tr"
   shows "ParValid P (Parallel p1 chs p2) Q"
   using ParValid_Parallel[OF assms(1,2)]
-  by (smt ParValid_def assms(3) assms(4) entails_def)
+  unfolding ParValid_def using assms(3,4) by blast
 
 
 subsection \<open>Simple examples\<close>
@@ -751,7 +795,7 @@ text \<open>Send 1\<close>
 lemma testHL1:
   "Valid
     (\<lambda>s tr. Q s (tr @ [OutBlock ''ch'' 1]) \<and>
-            (\<forall>d>0. Q s (tr @ [WaitBlock d (\<lambda>\<tau>\<in>{0..d}. s) ({''ch''}, {}), OutBlock ''ch'' 1])))
+            (\<forall>d>0. Q s (tr @ [WaitBlock d (\<lambda>\<tau>\<in>{0..d}. State s) ({''ch''}, {}), OutBlock ''ch'' 1])))
     (Cm (''ch''[!](\<lambda>_. 1)))
     Q"
   by (rule Valid_send)
@@ -759,11 +803,11 @@ lemma testHL1:
 text \<open>This implies the strongest postcondition form\<close>
 lemma testHL1':
   "Valid
-    (\<lambda>s tr. s = Map.empty \<and> tr = [])
+    (\<lambda>s tr. s = (\<lambda>_. 0) \<and> tr = [])
     (Cm (''ch''[!](\<lambda>_. 1)))
-    (\<lambda>s tr. s = Map.empty \<and>
+    (\<lambda>s tr. s = (\<lambda>_. 0) \<and>
             (tr = [OutBlock ''ch'' 1] \<or>
-             (\<exists>d>0. tr = [WaitBlock d (\<lambda>\<tau>\<in>{0..d}. Map.empty) ({''ch''}, {}), OutBlock ''ch'' 1])))"
+             (\<exists>d>0. tr = [WaitBlock d (\<lambda>\<tau>\<in>{0..d}. State (\<lambda>_. 0)) ({''ch''}, {}), OutBlock ''ch'' 1])))"
   apply (rule Valid_weaken_pre)
    prefer 2
    apply (rule Valid_send)
@@ -773,10 +817,10 @@ text \<open>Send 1, then send 2\<close>
 lemma testHL2:
   "Valid
     (\<lambda>s tr. (Q s ((tr @ [OutBlock ''ch'' 1]) @ [OutBlock ''ch'' 2]) \<and>
-             (\<forall>d>0. Q s ((tr @ [OutBlock ''ch'' 1]) @ [WaitBlock d (\<lambda>\<tau>\<in>{0..d}. s) ({''ch''}, {}), OutBlock ''ch'' 2]))) \<and>
-            (\<forall>d>0. Q s ((tr @ [WaitBlock d (\<lambda>\<tau>\<in>{0..d}. s) ({''ch''}, {}), OutBlock ''ch'' 1]) @ [OutBlock ''ch'' 2]) \<and>
-             (\<forall>da>0. Q s ((tr @ [WaitBlock d (\<lambda>\<tau>\<in>{0..d}. s) ({''ch''}, {}), OutBlock ''ch'' 1]) @
-                           [WaitBlock da (\<lambda>\<tau>\<in>{0..da}. s) ({''ch''}, {}), OutBlock ''ch'' 2]))))
+             (\<forall>d>0. Q s ((tr @ [OutBlock ''ch'' 1]) @ [WaitBlock d (\<lambda>\<tau>\<in>{0..d}. State s) ({''ch''}, {}), OutBlock ''ch'' 2]))) \<and>
+            (\<forall>d>0. Q s ((tr @ [WaitBlock d (\<lambda>\<tau>\<in>{0..d}. State s) ({''ch''}, {}), OutBlock ''ch'' 1]) @ [OutBlock ''ch'' 2]) \<and>
+             (\<forall>da>0. Q s ((tr @ [WaitBlock d (\<lambda>\<tau>\<in>{0..d}. State s) ({''ch''}, {}), OutBlock ''ch'' 1]) @
+                           [WaitBlock da (\<lambda>\<tau>\<in>{0..da}. State s) ({''ch''}, {}), OutBlock ''ch'' 2]))))
     (Cm (''ch''[!](\<lambda>_. 1)); Cm (''ch''[!](\<lambda>_. 2)))
     Q"
   apply (rule Valid_seq)
@@ -787,8 +831,8 @@ text \<open>Receive from ch\<close>
 lemma testHL3:
   "Valid
     (\<lambda>s tr.
-        (\<forall>v. Q (s(X \<mapsto> v)) (tr @ [InBlock ''ch'' v])) \<and>
-        (\<forall>d>0. \<forall>v. Q (s(X \<mapsto> v)) (tr @ [WaitBlock d (\<lambda>\<tau>\<in>{0..d}. s) ({}, {''ch''}), InBlock ''ch'' v])))
+        (\<forall>v. Q (s(X := v)) (tr @ [InBlock ''ch'' v])) \<and>
+        (\<forall>d>0. \<forall>v. Q (s(X := v)) (tr @ [WaitBlock d (\<lambda>\<tau>\<in>{0..d}. State s) ({}, {''ch''}), InBlock ''ch'' v])))
     (Cm (''ch''[?]X))
     Q"
   by (rule Valid_receive)
@@ -796,11 +840,11 @@ lemma testHL3:
 text \<open>Strongest postcondition form\<close>
 lemma testHL3':
   "Valid
-    (\<lambda>s tr. s = Map.empty \<and> tr = [])
+    (\<lambda>s tr. s = (\<lambda>_. 0) \<and> tr = [])
     (Cm (''ch''[?]X))
-    (\<lambda>s tr. (\<exists>v. s = [X \<mapsto> v] \<and>
+    (\<lambda>s tr. (\<exists>v. s = ((\<lambda>_. 0)(X := v)) \<and>
               (tr = [InBlock ''ch'' v]) \<or>
-               (\<exists>d>0. tr = [WaitBlock d (\<lambda>\<tau>\<in>{0..d}. Map.empty) ({}, {''ch''}), InBlock ''ch'' v])))"
+               (\<exists>d>0. tr = [WaitBlock d (\<lambda>\<tau>\<in>{0..d}. State (\<lambda>_. 0)) ({}, {''ch''}), InBlock ''ch'' v])))"
   apply (rule Valid_weaken_pre)
    prefer 2
    apply (rule testHL3)
@@ -809,16 +853,17 @@ lemma testHL3':
 text \<open>Communication\<close>
 lemma testHL4:
   "ParValid
-    (\<lambda>s. s = Map.empty)
-    (Parallel (Single {} (Cm (''ch''[!](\<lambda>_. 1)))) {''ch''}
-              (Single {X} (Cm (''ch''[?]X))))
-    (\<lambda>s tr. s |` {X} = [X \<mapsto> 1] \<and> tr = [IOBlock ''ch'' 1])"
+    (pair_assn (\<lambda>s. s = (\<lambda>_. 0)) (\<lambda>s. s = (\<lambda>_. 0)))
+    (Parallel (Single (Cm (''ch''[!](\<lambda>_. 1)))) {''ch''}
+              (Single (Cm (''ch''[?]X))))
+    (\<lambda>s tr. pair_assn (\<lambda>s. s = (\<lambda>_. 0)) (\<lambda>s. s = ((\<lambda>_. 0)(X := 1))) s \<and> tr = [IOBlock ''ch'' 1])"
   apply (rule ParValid_Parallel')
      apply (rule ParValid_Single[OF testHL1'])
     apply (rule ParValid_Single[OF testHL3'])
-   apply (auto simp add: entails_def)
+   apply (auto simp add: entails_def pair_assn_def par_assn_def sing_assn_def)
   by (auto elim!: combine_blocks_elim1 combine_blocks_elim2a combine_blocks_elim2b
-                  combine_blocks_elim2e combine_blocks_elim4a) 
+                  combine_blocks_elim2e combine_blocks_elim4a)
+  
 
 subsection \<open>Standard assertions\<close>
 
@@ -846,11 +891,11 @@ definition all_assn :: "(real \<Rightarrow> tassn) \<Rightarrow> tassn" (binder 
 
 inductive out_assn :: "state \<Rightarrow> cname \<Rightarrow> real \<Rightarrow> tassn" ("Out\<^sub>A") where
   "Out\<^sub>A s ch v [OutBlock ch v]"
-| "d > 0 \<Longrightarrow> Out\<^sub>A s ch v [WaitBlock d (\<lambda>\<tau>\<in>{0..d}. s) ({ch}, {}), OutBlock ch v]"
+| "d > 0 \<Longrightarrow> Out\<^sub>A s ch v [WaitBlock d (\<lambda>\<tau>\<in>{0..d}. State s) ({ch}, {}), OutBlock ch v]"
 
 inductive in_assn :: "state \<Rightarrow> cname \<Rightarrow> real \<Rightarrow> tassn" ("In\<^sub>A") where
   "In\<^sub>A s ch v [InBlock ch v]"
-| "d > 0 \<Longrightarrow> In\<^sub>A s ch v [WaitBlock d (\<lambda>\<tau>\<in>{0..d}. s) ({}, {ch}), InBlock ch v]"
+| "d > 0 \<Longrightarrow> In\<^sub>A s ch v [WaitBlock d (\<lambda>\<tau>\<in>{0..d}. State s) ({}, {ch}), InBlock ch v]"
 
 lemma emp_unit_left [simp]:
   "(emp\<^sub>A @\<^sub>t P) = P"
@@ -884,7 +929,7 @@ theorem Valid_send':
 
 theorem Valid_receive':
   "Valid
-    (\<lambda>s. \<forall>\<^sub>A v. ((In\<^sub>A s ch v) @- P (s(var := Some v))))
+    (\<lambda>s. \<forall>\<^sub>A v. ((In\<^sub>A s ch v) @- P (s(var := v))))
     (Cm (ch[?]var))
     P"
   apply (rule Valid_weaken_pre)
@@ -916,9 +961,9 @@ lemma testHL1s:
 text \<open>Strongest postcondition form\<close>
 lemma testHL1s':
   "Valid
-    (\<lambda>s tr. s = Map.empty \<and> P tr)
+    (\<lambda>s tr. s = (\<lambda>_. 0) \<and> P tr)
     (Cm (''ch''[!](\<lambda>_. 1)))
-    (\<lambda>s tr. s = Map.empty \<and> (P @\<^sub>t Out\<^sub>A s ''ch'' 1) tr)"
+    (\<lambda>s tr. s = (\<lambda>_. 0) \<and> (P @\<^sub>t Out\<^sub>A s ''ch'' 1) tr)"
   apply (rule Valid_weaken_pre)
    prefer 2 apply (rule testHL1s)
   unfolding entails_def apply simp
@@ -938,9 +983,9 @@ lemma testHL2s:
 text \<open>Strongest postcondition form\<close>
 lemma testHL2s':
   "Valid
-    (\<lambda>s tr. s = Map.empty \<and> P tr)
+    (\<lambda>s tr. s = (\<lambda>_. 0) \<and> P tr)
     (Cm (''ch''[!](\<lambda>_. 1)); Cm (''ch''[!](\<lambda>_. 2)))
-    (\<lambda>s tr. s = Map.empty \<and> (P @\<^sub>t (Out\<^sub>A s ''ch'' 1) @\<^sub>t (Out\<^sub>A s ''ch'' 2)) tr)"
+    (\<lambda>s tr. s = (\<lambda>_. 0) \<and> (P @\<^sub>t (Out\<^sub>A s ''ch'' 1) @\<^sub>t (Out\<^sub>A s ''ch'' 2)) tr)"
   apply (rule Valid_weaken_pre)
    prefer 2 apply (rule testHL2s)
   unfolding entails_def apply simp
@@ -953,7 +998,7 @@ lemma testHL2s':
 text \<open>Receive from ch\<close>
 lemma testHL3s:
   "Valid
-    (\<lambda>s. \<forall>\<^sub>Av. In\<^sub>A s ''ch'' v @- P (s(X \<mapsto> v)))
+    (\<lambda>s. \<forall>\<^sub>Av. In\<^sub>A s ''ch'' v @- P (s(X := v)))
     (Cm (''ch''[?]X))
     P"
   by (rule Valid_receive')
@@ -961,9 +1006,9 @@ lemma testHL3s:
 text \<open>Strongest postcondition form\<close>
 lemma testHL3s':
   "Valid
-    (\<lambda>s tr. s = Map.empty \<and> P tr)
+    (\<lambda>s tr. s = (\<lambda>_. 0) \<and> P tr)
     (Cm (''ch''[?]X))
-    (\<lambda>s tr. \<exists>v. s = [X \<mapsto> v] \<and> (P @\<^sub>t In\<^sub>A (Map.empty) ''ch'' v) tr)"
+    (\<lambda>s tr. \<exists>v. s = ((\<lambda>_. 0)(X := v)) \<and> (P @\<^sub>t In\<^sub>A (\<lambda>_. 0) ''ch'' v) tr)"
   apply (rule Valid_weaken_pre)
    prefer 2 apply (rule testHL3s)
   unfolding entails_def
@@ -972,7 +1017,7 @@ lemma testHL3s':
 text \<open>Receive two values in a row\<close>
 lemma testHL3a:
   "Valid
-    ((\<lambda>s. \<forall>\<^sub>Av. In\<^sub>A s ''ch'' v @- (\<forall>\<^sub>Aw. In\<^sub>A (s(X \<mapsto> v)) ''ch'' w @- P (s(X \<mapsto> w)))))
+    ((\<lambda>s. \<forall>\<^sub>Av. In\<^sub>A s ''ch'' v @- (\<forall>\<^sub>Aw. In\<^sub>A (s(X := v)) ''ch'' w @- P (s(X := w)))))
     (Cm (''ch''[?]X); Cm (''ch''[?]X))
     P"
   apply (rule Valid_weaken_pre) prefer 2
@@ -984,9 +1029,9 @@ lemma testHL3a:
 text \<open>Strongest postcondition form\<close>
 lemma testHL3a':
   "Valid
-    (\<lambda>s tr. s = Map.empty \<and> P tr)
+    (\<lambda>s tr. s = (\<lambda>_. 0) \<and> P tr)
     (Cm (''ch''[?]X); Cm (''ch''[?]X))
-    (\<lambda>s tr. \<exists>v w. s = [X \<mapsto> w] \<and> (P @\<^sub>t In\<^sub>A (Map.empty) ''ch'' v @\<^sub>t In\<^sub>A [X \<mapsto> v] ''ch'' w) tr)"
+    (\<lambda>s tr. \<exists>v w. s = ((\<lambda>_. 0)(X := w)) \<and> (P @\<^sub>t In\<^sub>A (\<lambda>_. 0) ''ch'' v @\<^sub>t In\<^sub>A ((\<lambda>_. 0)(X := v)) ''ch'' w) tr)"
   apply (rule Valid_weaken_pre)
    prefer 2 apply (rule Valid_seq)
     prefer 2 apply (rule Valid_receive')
@@ -998,14 +1043,14 @@ lemma testHL3a':
 text \<open>Communication\<close>
 lemma testHL4s:
   "ParValid
-    (\<lambda>s. s = Map.empty)
-    (Parallel (Single {} (Cm (''ch''[!](\<lambda>_. 1)))) {''ch''}
-              (Single {X} (Cm (''ch''[?]X))))
-    (\<lambda>s tr. s |` {X} = [X \<mapsto> 1] \<and> tr = [IOBlock ''ch'' 1])"
+    (pair_assn (\<lambda>s. s = (\<lambda>_. 0)) (\<lambda>s. s = (\<lambda>_. 0)))
+    (Parallel (Single (Cm (''ch''[!](\<lambda>_. 1)))) {''ch''}
+              (Single (Cm (''ch''[?]X))))
+    (\<lambda>s tr. pair_assn (\<lambda>s. s = (\<lambda>_. 0)) (\<lambda>s. s = ((\<lambda>_. 0)(X := 1))) s \<and> tr = [IOBlock ''ch'' 1])"
   apply (rule ParValid_Parallel')
      apply (rule ParValid_Single[OF testHL1s'[where P="emp\<^sub>A"]])
     apply (rule ParValid_Single[OF testHL3s'[where P="emp\<^sub>A"]])
-   apply (auto simp add: entails_def)
+   apply (auto simp add: entails_def pair_assn_def par_assn_def sing_assn_def)
   by (auto simp add: emp_assn_def elim!: combine_assn_elim2)
 
 
@@ -1014,13 +1059,13 @@ subsection \<open>Examples for loops\<close>
 text \<open>First example simply counts up variable X.\<close>
 fun count_up_inv :: "nat \<Rightarrow> tassn" where
   "count_up_inv 0 = emp\<^sub>A"
-| "count_up_inv (Suc n) = count_up_inv n @\<^sub>t Out\<^sub>A [X \<mapsto> n] ''ch'' n"
+| "count_up_inv (Suc n) = count_up_inv n @\<^sub>t Out\<^sub>A ((\<lambda>_. 0)(X := real n)) ''ch'' n"
 
 lemma testLoop1:
   "Valid
-    (\<lambda>s tr. s = [X \<mapsto> a] \<and> count_up_inv a tr)
-    (Rep (Cm (''ch''[!](\<lambda>s. the (s X))); Assign X (\<lambda>s. the (s X) + 1)))
-    (\<lambda>s tr. \<exists>n. n \<ge> a \<and> s = [X \<mapsto> n] \<and> count_up_inv n tr)"
+    (\<lambda>s tr. s = ((\<lambda>_. 0)(X := a)) \<and> count_up_inv a tr)
+    (Rep (Cm (''ch''[!](\<lambda>s. s X)); Assign X (\<lambda>s. s X + 1)))
+    (\<lambda>s tr. \<exists>n. n \<ge> a \<and> s = ((\<lambda>_. 0)(X := n)) \<and> count_up_inv n tr)"
   apply (rule Valid_weaken_pre)
    prefer 2 apply (rule Valid_rep)
    apply (rule Valid_weaken_pre)
@@ -1037,13 +1082,13 @@ lemma testLoop1:
 text \<open>In each iteration, increment by 1, output, then increment by 2.\<close>
 fun count_up3_inv1 :: "nat \<Rightarrow> tassn" where
   "count_up3_inv1 0 = emp\<^sub>A"
-| "count_up3_inv1 (Suc n) = count_up3_inv1 n @\<^sub>t Out\<^sub>A [X \<mapsto> 3 * n + 1] ''ch'' (3 * n + 1)"
+| "count_up3_inv1 (Suc n) = count_up3_inv1 n @\<^sub>t Out\<^sub>A ((\<lambda>_. 0)(X := 3 * real n + 1)) ''ch'' (3 * real n + 1)"
 
 lemma testLoop2:
   "Valid
-    (\<lambda>s tr. s = [X \<mapsto> 3 * a] \<and> count_up3_inv1 a tr)
-    (Rep (Assign X (\<lambda>s. the (s X) + 1); Cm (''ch''[!](\<lambda>s. the (s X))); Assign X (\<lambda>s. the (s X) + 2)))
-    (\<lambda>s tr. \<exists>n. n \<ge> a \<and> s = [X \<mapsto> 3 * n] \<and> count_up3_inv1 n tr)"
+    (\<lambda>s tr. s = ((\<lambda>_. 0)(X := 3 * a)) \<and> count_up3_inv1 a tr)
+    (Rep (Assign X (\<lambda>s. s X + 1); Cm (''ch''[!](\<lambda>s. s X)); Assign X (\<lambda>s. s X + 2)))
+    (\<lambda>s tr. \<exists>n. n \<ge> a \<and> s = ((\<lambda>_. 0)(X := 3 * n)) \<and> count_up3_inv1 n tr)"
   apply (rule Valid_weaken_pre)
    prefer 2 apply (rule Valid_rep)
   apply (rule Valid_weaken_pre)
@@ -1062,15 +1107,15 @@ subsection \<open>Test cases for external choice\<close>
 
 inductive inrdy_assn :: "state \<Rightarrow> cname \<Rightarrow> real \<Rightarrow> rdy_info \<Rightarrow> tassn" ("Inrdy\<^sub>A") where
   "Inrdy\<^sub>A s ch v rdy [InBlock ch v]"
-| "d > 0 \<Longrightarrow> Inrdy\<^sub>A s ch v rdy [WaitBlock d (\<lambda>\<tau>\<in>{0..d}. s) rdy, InBlock ch v]"
+| "d > 0 \<Longrightarrow> Inrdy\<^sub>A s ch v rdy [WaitBlock d (\<lambda>\<tau>\<in>{0..d}. State s) rdy, InBlock ch v]"
 
 text \<open>First, we restate the rule for Valid_echoice in simpler form\<close>
 theorem Valid_echoice_InIn':
   assumes "Valid Q1 p1 R"
     and "Valid Q2 p2 R"
   shows "Valid
-    (\<lambda>s. (\<forall>\<^sub>Av. ((Inrdy\<^sub>A s ch1 v ({}, {ch1, ch2})) @- Q1 (s(var1 := Some v)))) \<and>\<^sub>A
-         (\<forall>\<^sub>Av. ((Inrdy\<^sub>A s ch2 v ({}, {ch1, ch2})) @- Q2 (s(var2 := Some v)))))
+    (\<lambda>s. (\<forall>\<^sub>Av. ((Inrdy\<^sub>A s ch1 v ({}, {ch1, ch2})) @- Q1 (s(var1 := v)))) \<and>\<^sub>A
+         (\<forall>\<^sub>Av. ((Inrdy\<^sub>A s ch2 v ({}, {ch1, ch2})) @- Q2 (s(var2 := v)))))
       (EChoice [(ch1[?]var1, p1), (ch2[?]var2, p2)])
     R"
   apply (rule Valid_weaken_pre)
@@ -1080,8 +1125,8 @@ theorem Valid_echoice_InIn':
 
 lemma echoice_test1:
   "Valid
-    (\<lambda>s. (\<forall>\<^sub>Av. ((Inrdy\<^sub>A s ''ch1'' v ({}, {''ch1'', ''ch2''})) @- Q (s(X \<mapsto> v)))) \<and>\<^sub>A
-         (\<forall>\<^sub>Av. ((Inrdy\<^sub>A s ''ch2'' v ({}, {''ch1'', ''ch2''})) @- Q (s(X \<mapsto> v)))))
+    (\<lambda>s. (\<forall>\<^sub>Av. ((Inrdy\<^sub>A s ''ch1'' v ({}, {''ch1'', ''ch2''})) @- Q (s(X := v)))) \<and>\<^sub>A
+         (\<forall>\<^sub>Av. ((Inrdy\<^sub>A s ''ch2'' v ({}, {''ch1'', ''ch2''})) @- Q (s(X := v)))))
     (EChoice [(''ch1''[?]X, Skip), (''ch2''[?]X, Skip)])
     Q"
   apply (rule Valid_echoice_InIn')
@@ -1091,10 +1136,10 @@ lemma echoice_test1:
 text \<open>Strongest postcondition form\<close>
 lemma echoice_test1':
   "Valid
-    (\<lambda>s tr. s = Map.empty \<and> P tr)
+    (\<lambda>s tr. s = (\<lambda>_. 0) \<and> P tr)
     (EChoice [(''ch1''[?]X, Skip), (''ch2''[?]X, Skip)])
-    (\<lambda>s tr. (\<exists>v. s = [X \<mapsto> v] \<and> (P @\<^sub>t Inrdy\<^sub>A (Map.empty) ''ch1'' v ({}, {''ch1'', ''ch2''})) tr) \<or>
-            (\<exists>v. s = [X \<mapsto> v] \<and> (P @\<^sub>t Inrdy\<^sub>A (Map.empty) ''ch2'' v ({}, {''ch1'', ''ch2''})) tr))"
+    (\<lambda>s tr. (\<exists>v. s = ((\<lambda>_. 0)(X := v)) \<and> (P @\<^sub>t Inrdy\<^sub>A (\<lambda>_. 0) ''ch1'' v ({}, {''ch1'', ''ch2''})) tr) \<or>
+            (\<exists>v. s = ((\<lambda>_. 0)(X := v)) \<and> (P @\<^sub>t Inrdy\<^sub>A (\<lambda>_. 0) ''ch2'' v ({}, {''ch1'', ''ch2''})) tr))"
   apply (rule Valid_weaken_pre)
    prefer 2 apply (rule echoice_test1)
   apply (auto simp add: entails_def and_assn_def magic_wand_assn_def join_assn_def all_assn_def)
@@ -1108,8 +1153,8 @@ lemma echoice_test1':
 text \<open>Contrast this with the case of internal choice\<close>
 lemma ichoice_test1:
   "Valid
-    (\<lambda>s. (\<forall>\<^sub>Av. In\<^sub>A s ''ch1'' v @- Q (s(X \<mapsto> v))) \<and>\<^sub>A
-         (\<forall>\<^sub>Av. In\<^sub>A s ''ch2'' v @- Q (s(X \<mapsto> v))))
+    (\<lambda>s. (\<forall>\<^sub>Av. In\<^sub>A s ''ch1'' v @- Q (s(X := v))) \<and>\<^sub>A
+         (\<forall>\<^sub>Av. In\<^sub>A s ''ch2'' v @- Q (s(X := v))))
     (IChoice (Cm (''ch1''[?]X)) (Cm (''ch2''[?]X)))
     Q"
   apply (rule Valid_weaken_pre)
@@ -1120,10 +1165,10 @@ lemma ichoice_test1:
 text \<open>Strongest postcondition form\<close>
 lemma ichoice_test1':
   "Valid
-    (\<lambda>s tr. s = Map.empty \<and> P tr)
+    (\<lambda>s tr. s = (\<lambda>_. 0) \<and> P tr)
     (IChoice (Cm (''ch1''[?]X)) (Cm (''ch2''[?]X)))
-    (\<lambda>s tr. (\<exists>v. s = [X \<mapsto> v] \<and> (P @\<^sub>t In\<^sub>A (Map.empty) ''ch1'' v) tr) \<or>
-            (\<exists>v. s = [X \<mapsto> v] \<and> (P @\<^sub>t In\<^sub>A (Map.empty) ''ch2'' v) tr))"
+    (\<lambda>s tr. (\<exists>v. s = ((\<lambda>_. 0)(X := v)) \<and> (P @\<^sub>t In\<^sub>A (\<lambda>_. 0) ''ch1'' v) tr) \<or>
+            (\<exists>v. s = ((\<lambda>_. 0)(X := v)) \<and> (P @\<^sub>t In\<^sub>A (\<lambda>_. 0) ''ch2'' v) tr))"
   apply (rule Valid_weaken_pre)
    prefer 2 apply (rule ichoice_test1)
   apply (auto simp add: entails_def and_assn_def magic_wand_assn_def join_assn_def all_assn_def)
